feat: use class predicate and impl add op

set.dfy
@@ -1,30 +1,58 @@
 // Bernardo Zomer, Carlo Mantovani and Lucas Cunha
 
 // An array-based set of elements of type int.
-class Set {
+class {:autocontracts true} Set {
     var elements: array<int>
+    var size: int
 
-    constructor() {
+    ghost var ghostElements: seq<int>
+    ghost var ghostSize: int
+
+    ghost predicate Valid() {
+        this.ghostElements == this.elements[..]
+        && this.ghostSize == this.size
+        && this.size == this.elements.Length
+    }
+
+    constructor() 
+        ensures this.ghostElements == []
+        ensures this.ghostSize == 0
+    {
         this.elements := new int[0];
+        this.size := 0;
+        this.ghostElements := [];
+        this.ghostSize := 0;
     }
 
     // Ensures an element is in the set
     // and returns true if it was previously not present.
     method Add(e: int) returns (isNewElement: bool)
-        modifies this.elements
         // Ensures the element will be in the set.
         ensures e in this.elements[..]
         ensures isNewElement ==>
             // Ensures the element was not present in the set if isNewElement is true.
-            !(e in old(this.elements[..]))
-            // Ensures the first n elements of the element array were not changed, 
-            // where n is the length of the old array.
-            && this.elements[0..old(this.elements.Length)] == old(this.elements[..]) 
-            // Ensures the last index of the element array contains the element.
-            && this.elements[this.elements.Length - 1] == e
+            !(old(Contains(e)))
+            // Ensures the array is the same as before 
+            // with the added element at the end.
+            && this.ghostElements == old(this.ghostElements) + [e]
+            && this.ghostSize == old(this.ghostSize + 1)
         // Ensures the element array has not been changed 
         // if the element was already present in the set.
-        ensures !isNewElement ==> this.elements == old(this.elements)
+        ensures !isNewElement ==> this.ghostElements == old(this.ghostElements)
+        ensures Valid()
+    {
+        isNewElement := !Contains(e);
+
+        if isNewElement {
+            var newElements := new int[this.size + 1];
+            forall i | 0 <= i < size { newElements[i] := this.elements[i]; }
+            newElements[this.size] := e;
+            this.elements := newElements;
+            this.size := this.size + 1;
+            this.ghostElements := this.elements[..];
+            this.ghostSize := this.size;
+        }
+    }
 
     // Ensures an element is not in the set
     // and returns true if it was previously present.
@@ -39,29 +67,23 @@ class Set {
         ensures !wasInSet ==> this.elements == old(this.elements)
 
     // Returns whether the set contains an element or not.
-    method Contains(e: int) returns (contains: bool)
-        ensures contains ==> e in this.elements[..]
+    function Contains(e: int): bool
+        ensures Valid()
     {
-        for i := 0 to this.elements.Length {
-            if this.elements[i] == e {
-                return true;
-            }
-        }
-
-        return false;
+        e in this.elements[..]
     }
 
     // Returns the amount of elements in the set.
-    method Size() returns (length: int)
-        ensures length == this.elements.Length
+    function Size(): int
+        ensures Valid()
     {
-        return this.elements.Length;
+        this.size
     }
 
     // Returns whether the set is empty or not.
-    method IsEmpty() returns (isEmpty: bool)
-        ensures isEmpty ==> this.elements.Length == 0
+    function IsEmpty(): bool
+        ensures Valid()
     {
-        return this.elements.Length == 0;
+        this.size == 0
     }
 }
